secd/ssr_msecd_1_db.v
@@ -193,9 +193,9 @@ Section MiniMLdB.
       case: (IH2 o He d2 H8) => v2' [H21 H22] {IH2}. (* 引数部 *)
       
       (* クロージャの中身を評価する環境 *)
-      Check (VClosRec f x e3 g3).
+      Check (uClosRec f x e3 g3).
       have He3 : dB_translation_NS_env
-                   ((x, v2) :: (f, (VClosRec f x e3 g3)) :: g3)
+                   ((x, v2) :: (f, (uClosRec f x e3 g3)) :: g3)
                    (v2' :: (vClosRec d o0) :: o0).
       + apply: dB_translation_NS_env_cons.
         * apply: dB_translation_NS_env_cons.
@@ -206,7 +206,7 @@ Section MiniMLdB.
       (* クロージャの中身を変換する。 *)
       Check (IH3 (v2' :: (vClosRec d o0) :: o0) He3 d).
       have H30 : dB_translation_NS
-                   (mkctx ((x, v2) :: (f, VClosRec f x e3 g3) :: g3)) e3 d
+                   (mkctx ((x, v2) :: (f, uClosRec f x e3 g3) :: g3)) e3 d
         by apply: H13.
       
       Check (IH3 (v2' :: (vClosRec d o0) :: o0) He3 d H30).
@@ -225,11 +225,11 @@ Section MiniMLdB.
   (* ***************************************** *)
   (* ***************************************** *)
   
-  Theorem dB_translation_NS_correctness g t v :
-    MML_NS g t v ->
+  Theorem dB_translation_NS_correctness g t u :
+    MML_NS g t u ->
     forall o, dB_translation_NS_env g o ->
               forall d, dB_translation_NS (mkctx g) t d ->
-                        exists vd, dB_translation_NS_val v vd /\ MML_dB_NS o d vd.
+                        exists v, dB_translation_NS_val u v /\ MML_dB_NS o d v.
   Proof.
     elim.
     (* Nat *)
@@ -247,9 +247,9 @@ Section MiniMLdB.
     (* Plus *)
     - move=> g' t1 t2 m n H1 IH1 H2 IH2 o He d H.
       inv: H => H5 H7.
-      case: (IH1 o He d1 H5) => vd1 [H11 H12].
+      case: (IH1 o He d1 H5) => v1 [H11 H12].
       inv: H11.
-      case: (IH2 o He d2 H7) => vd2 [H21 H22].
+      case: (IH2 o He d2 H7) => v2 [H21 H22].
       inv: H21.
       exists (vNat (m + n)).
       split => //.
@@ -258,9 +258,9 @@ Section MiniMLdB.
     (* Minus *)
     - move=> g' t1 t2 m n H1 IH1 H2 IH2 o He d H.
       inv: H => H5 H7.
-      case: (IH1 o He d1 H5) => vd1 [H11 H12].
+      case: (IH1 o He d1 H5) => v1 [H11 H12].
       inv: H11.
-      case: (IH2 o He d2 H7) => vd2 [H21 H22].
+      case: (IH2 o He d2 H7) => v2 [H21 H22].
       inv: H21.
       exists (vNat (m - n)).
       split => //.
@@ -269,9 +269,9 @@ Section MiniMLdB.
     (* Times *)
     - move=> g' t1 t2 m n H1 IH1 H2 IH2 o He d H.
       inv: H => H5 H7.
-      case: (IH1 o He d1 H5) => vd1 [H11 H12].
+      case: (IH1 o He d1 H5) => v1 [H11 H12].
       inv: H11.
-      case: (IH2 o He d2 H7) => vd2 [H21 H22].
+      case: (IH2 o He d2 H7) => v2 [H21 H22].
       inv: H21.
       exists (vNat (m * n)).
       split => //.
@@ -290,24 +290,24 @@ Section MiniMLdB.
       + by [].
         
     (* Let *)
-    - move=> g' x g1 g2 v1 v2 H1 IH1 H2 IH2 o He d H.
+    - move=> g' x g1 g2 u1 u2 H1 IH1 H2 IH2 o He d H.
       inv: H => H7 H8.
-      case: (IH1 o He d1 H7) => vd1 [H11 H12].
-      have He2 : dB_translation_NS_env ((x, v1) :: g') (vd1 :: o)
+      case: (IH1 o He d1 H7) => v1 [H11 H12].
+      have He2 : dB_translation_NS_env ((x, u1) :: g') (v1 :: o)
         by apply: dB_translation_NS_env_cons.
-      have H82 : dB_translation_NS (mkctx ((x, v1) :: g')) g2 d2 by apply: H8.
-      case: (IH2 (vd1 :: o) He2 d2 H82) => vd2 [H21 H22].
-      exists vd2.
+      have H82 : dB_translation_NS (mkctx ((x, u1) :: g')) g2 d2 by apply: H8.
+      case: (IH2 (v1 :: o) He2 d2 H82) => v2 [H21 H22].
+      exists v2.
       split=> //.
-        by apply: (MML_dB_NS_Let o d1 d2 vd1 vd2).
+        by apply: (MML_dB_NS_Let o d1 d2 v1 v2).
         
     (* If true *)
-    - move=> g' t1 t2 t3 v2 H1 IH1 H2 IH2 o He d H.
+    - move=> g' t1 t2 t3 u2 H1 IH1 H2 IH2 o He d H.
       inv: H => H6 H8 H9.
-      case: (IH1 o He d1 H6) => vd1 [H11 H12].
+      case: (IH1 o He d1 H6) => v1 [H11 H12].
       inv: H11.
-      case: (IH2 o He d2 H8) => vd2 [H21 H22].
-      exists vd2.
+      case: (IH2 o He d2 H8) => v2 [H21 H22].
+      exists v2.
       split=> //.
       apply: MML_dB_NS_Iftrue.
       invs: H12 => [m n H0 H5 H].
@@ -315,12 +315,12 @@ Section MiniMLdB.
       + by [].
         
     (* If false *)
-    - move=> g' t1 t2 t3 v3 H1 IH1 H3 IH3 o He d H.
+    - move=> g' t1 t2 t3 u3 H1 IH1 H3 IH3 o He d H.
       inv: H => H6 H8 H9.
-      case: (IH1 o He d1 H6) => vd1 [H11 H12].
+      case: (IH1 o He d1 H6) => v1 [H11 H12].
       inv: H11.
-      case: (IH3 o He d3 H9) => vd3 [H31 H32].
-      exists vd3.
+      case: (IH3 o He d3 H9) => v3 [H31 H32].
+      exists v3.
       split=> //.
       apply: MML_dB_NS_Iffalse.
       invs: H12 => [m n H0 H5 H].
@@ -344,35 +344,35 @@ Section MiniMLdB.
       + by [].
         
     (* App Clos *)
-    - move=> g' g3 x t1 t2 t3 v2 v3 H1 IH1 H2 IH2 H3 IH3 o He d H.
+    - move=> g' g3 x t1 t2 t3 u2 v3 H1 IH1 H2 IH2 H3 IH3 o He d H.
       inv: H => H6 H8.
-      case: (IH1 o He d1 H6) => vd1 [H11 H12] {IH1}. (* 関数部 *)
+      case: (IH1 o He d1 H6) => v1 [H11 H12] {IH1}. (* 関数部 *)
       inv: H11 => H9 H10.
-      case: (IH2 o He d2 H8) => vd2 [H21 H22] {IH2}. (* 引数部 *)
+      case: (IH2 o He d2 H8) => v2 [H21 H22] {IH2}. (* 引数部 *)
       (* クロージャの中身を評価する環境 *)
-      have He3 : dB_translation_NS_env ((x, v2) :: g3) (vd2 :: o0)
+      have He3 : dB_translation_NS_env ((x, u2) :: g3) (v2 :: o0)
         by apply: dB_translation_NS_env_cons.
       (* クロージャの中身を変換する。 *)
-      have H30 : dB_translation_NS (mkctx ((x, v2) :: g3)) t3 d by apply: H10.
-      case: (IH3 (vd2 :: o0) He3 d H30) => vd3 [H31 H32] {IH3}.
-      exists vd3.
+      have H30 : dB_translation_NS (mkctx ((x, u2) :: g3)) t3 d by apply: H10.
+      case: (IH3 (v2 :: o0) He3 d H30) => u3 [H31 H32] {IH3}.
+      exists u3.
       split=> //.
         by apply: MML_dB_NS_App; [apply: H12 | apply: H22 | apply: H32].
         
     (* App ClosRec *)
-    - move=> g' g3 x f t1 t2 t3 v2 v3 H1 IH1 H2 IH2 H3 IH3 o He d H.
+    - move=> g' g3 x f t1 t2 t3 u2 v3 H1 IH1 H2 IH2 H3 IH3 o He d H.
       inv: H => H6 H8.
-      case: (IH1 o He d1 H6) => vd1 [H11 H12] {IH1}.
+      case: (IH1 o He d1 H6) => v1 [H11 H12] {IH1}.
       move: (H11); inv=> H10 H13.           (* keepのために duplicate する。 *)
-      case: (IH2 o He d2 H8) => vd2 [H21 H22] {IH2}.
+      case: (IH2 o He d2 H8) => v2 [H21 H22] {IH2}.
       have He3 : dB_translation_NS_env
-                   ((x, v2) :: (f, (VClosRec f x t3 g3)) :: g3)
-                   (vd2 :: (vClosRec d o0) :: o0)
+                   ((x, u2) :: (f, (uClosRec f x t3 g3)) :: g3)
+                   (v2 :: (vClosRec d o0) :: o0)
         by apply: dB_translation_NS_env_cons; [apply: dB_translation_NS_env_cons |].
       have H30 : dB_translation_NS
-                   (mkctx ((x, v2) :: (f, VClosRec f x t3 g3) :: g3)) t3 d by [].
-      case: (IH3 (vd2 :: (vClosRec d o0) :: o0) He3 d H30) => vd3 [H31 H32] {IH3}.
-      exists vd3.
+                   (mkctx ((x, u2) :: (f, uClosRec f x t3 g3) :: g3)) t3 d by [].
+      case: (IH3 (v2 :: (vClosRec d o0) :: o0) He3 d H30) => u3 [H31 H32] {IH3}.
+      exists u3.
       split=> //.
         by apply: MML_dB_NS_AppRec; [apply: H12 | apply: H22 | apply: H32].
   Qed.
